- Adding my implementation

coq/Morello.v
@@ -2,500 +2,697 @@ Require Import Coq.Arith.PeanoNat.
 Require Import Coq.Lists.List.
 Require Import Coq.Strings.String.
 Require Import Coq.Strings.Ascii.
-Require Import Coq.Numbers.BinNums.
-Require Import Coq.ZArith.Zcompare.
 Require Import Coq.ZArith.Zdigits.
-Require Import Coq.Bool.Bool.
+Require Import Coq.Vectors.VectorDef.
+Require Import Coq.Bool.IfProp.
 
-Require Import StructTact.StructTactics.
+From stdpp.unstable Require Import bitvector. 
+Require Import Sail.Values.
+Require Import Sail.Prompt_monad.
+Require Import Sail.Operators_mwords.
+Require Import specCapFns.capfns_no_monad.
 
-Require Import bbv.Word.
+Require Import machine_capability.
+Require Import machine_address.
 
-From Sail Require  Import Base Impl_base Values Operators_mwords.
 
-Require Import Addr Capabilities Utils CapFns.
+(* Notations and their definitions*)
 
-Import ListNotations.
-Open Scope list_scope.
+(* Notation "x =? y" := (bool_decide (x = y)) (at level 70, no associativity) . *)
+Definition eq {n} (v1:bv n) (v2:bv n) : bool :=
+    v1.(bv_unsigned) =? v2.(bv_unsigned).
+Notation "x =? y" := (eq x y) (at level 70, no associativity).
+Definition lt {n} (v1:bv n) (v2:bv n) : bool :=
+    v1.(bv_unsigned) <? v2.(bv_unsigned).
+Notation "x <? y" := (lt x y) (at level 70, no associativity).
+Notation "x <=? y" := ((x <? y) || (x =? y)).
+Notation "x >? y" := (y <? x).
 
-Module MorelloAddr <: VADDR.
-  Definition t := Z. (* but it is always non-negiative *)
+Notation "(<@{ A } )" := (@lt A) (only parsing) : stdpp_scope.
+Notation LtDecision A := (RelDecision (<@{A})).
 
-  Definition sizeof_vaddr : nat := 8.
-  Definition vaddr_bits : nat := Nat.mul sizeof_vaddr 8%nat.
+Definition eqb_ADDR (n m : bv 64) : bool := (n =? m)%stdpp.
+Definition ltb_ADDR (n m : bv 64) : bool := (n.(bv_unsigned) <? m.(bv_unsigned))%Z.
+Definition lte_ADDR (n m : bv 64) : bool := eqb_ADDR n m || ltb_ADDR n m.
+Definition ltb_ADDR_irrefl (n : bv 64) := Z.ltb_irrefl n.(bv_unsigned).
 
-  Definition bitwise_complement (a:Z) :=
-    let bits := Z_to_binary vaddr_bits a in
+(** Utility convertors **)
+
+Definition bv_to_mword {n} (b : bv n) : mword (Z.of_N n) :=
+  mword_of_int (b.(bv_unsigned)).
+Definition bv_to_Z_unsigned {n} (v : bv n) : Z := v.(bv_unsigned).
+Definition bv_to_bv {n} {m : N} (v : bv n) : (bv m) :=
+  Z_to_bv m (bv_to_Z_unsigned v).
+Definition bv_to_list_bool {n} (v : bv n) : list bool := bv_to_bits v. 
+
+Definition mword_to_Z_unsigned {n} (m : mword n) : Z := int_of_mword false m.
+Definition mword_to_N {n} (m : mword n) : N := Z.to_N (int_of_mword false m).
+Definition mword_to_bv {n} (m : mword n) : bv (Z.to_N n) :=
+  Z_to_bv (Z.to_N n) (mword_to_Z_unsigned m). 
+
+Definition mword_to_bv_2 {z:Z} {n:N} (m : mword z)  : bv n :=
+  let x : Z := mword_to_Z_unsigned m in 
+  Z_to_bv n x.
+
+  Definition mword_to_list_bool {n} (w : mword n) : list bool := 
+  bitlistFromWord (get_word w). 
+
+Definition N_to_mword (m n : N) : mword (Z.of_N m) := 
+  mword_of_int (Z.of_N n).
+Program Definition list_bool_to_bv (l : list bool) : bv (N.of_nat (List.length l)) := 
+  @mword_to_bv (Z.of_nat (List.length l)) (of_bools (List.rev l)).
+ Next Obligation. intros. unfold Z.of_nat. destruct (base.length l). 
+ {reflexivity. } {reflexivity. } Defined.  
+Definition N_to_nat (n:N) : nat := (Z.to_nat (Z.of_N n)).
+
+Module tests_convertors.
+  Example converters_sound_1 : Z_to_bv 3 5 = mword_to_bv (bv_to_mword (Z_to_bv 3 5)).
+  Proof. reflexivity. Qed. 
+  Example converters_sound_2 : Z_to_bv 11 1000 = mword_to_bv (bv_to_mword (Z_to_bv 11 1000)).
+  Proof. reflexivity. Qed. 
+  Example converters_sound_3 : N_to_mword 12 2049 = bv_to_mword (mword_to_bv (N_to_mword 12 2049)).
+  Proof. reflexivity. Qed. 
+  Definition max_value : N := 680564733841876926926749214863536422911. (* 2^129 - 1 *)
+  Example converters_sound_4 : N_to_mword 129 max_value = bv_to_mword (mword_to_bv (N_to_mword 129 max_value)).
+  Proof. reflexivity. Qed. 
+  Example converters_sound_5 : Z_to_bv 129 (Z.of_N max_value) = mword_to_bv (bv_to_mword (Z_to_bv 129 (Z.of_N max_value))).
+  Proof. reflexivity. Qed.
+End tests_convertors. 
+
+Module Permissions <: Permission.
+  Definition len:N := 18. (* CAP_PERMS_NUM_BITS = 16 bits of actual perms + 2 bits for Executive and Global. *)
+  Definition t := bv len. 
+  
+  Definition to_Z (perms:t) : Z := bv_to_Z_unsigned perms.
+  Definition of_Z (z:Z) : t := Z_to_bv len z.
+  Program Definition of_list_bool (l:list bool)
+  `{(N.of_nat (List.length l) = len)%N} : t :=
+    list_bool_to_bv l.
+  Next Obligation. intros. apply H. Defined.
+
+  Definition user_perms_len:nat := 4.
+
+  Variant perm := Load_perm | Store_perm | Execute_perm | LoadCap_perm | StoreCap_perm | StoreLocalCap_perm | Seal_perm | Unseal_perm
+  | System_perm | BranchSealedPair_perm | CompartmentID_perm | MutableLoad_perm | User1_perm | User2_perm | User3_perm | User4_perm | Executive_perm | Global_perm.
+
+  Definition has_perm (permissions:t) : _ -> bool :=
+    let perms : (mword 64) := zero_extend (bv_to_mword permissions) 64 in 
+    fun perm => CapPermsInclude perms perm.
+
+  Definition has_global_perm (permissions:t) : bool := 
+    has_perm permissions CAP_PERM_GLOBAL.
+  Definition has_executive_perm (permissions:t) : bool := 
+    has_perm permissions CAP_PERM_EXECUTIVE.
+  Definition has_execute_perm (permissions:t) : bool := 
+    has_perm permissions CAP_PERM_EXECUTE.
+  Definition has_load_perm (permissions:t) : bool := 
+    has_perm permissions CAP_PERM_LOAD.
+  Definition has_load_cap_perm (permissions:t) : bool := 
+    has_perm permissions CAP_PERM_LOAD_CAP.
+  Definition has_seal_perm (permissions:t) : bool := 
+    has_perm permissions CAP_PERM_SEAL.
+  Definition has_store_perm (permissions:t) : bool := 
+    has_perm permissions CAP_PERM_STORE.
+  Definition has_store_cap_perm (permissions:t) : bool := 
+    has_perm permissions CAP_PERM_STORE_CAP.
+  Definition has_store_local_cap_perm (permissions:t) : bool := 
+    has_perm permissions CAP_PERM_STORE_LOCAL.
+  Definition has_system_access_perm (permissions:t) : bool := 
+    has_perm permissions CAP_PERM_SYSTEM.
+  Definition has_unseal_perm (permissions:t) : bool := 
+    has_perm permissions CAP_PERM_UNSEAL.
+  Definition has_user1_perm (permissions:t) : bool := 
+    has_perm permissions CAP_PERM_USER1.
+  Definition has_user2_perm (permissions:t) : bool := 
+    has_perm permissions CAP_PERM_USER2.
+  Definition has_user3_perm (permissions:t) : bool := 
+    has_perm permissions CAP_PERM_USER3.
+  Definition has_user4_perm (permissions:t) : bool := 
+    has_perm permissions CAP_PERM_USER4.
+  Definition has_compartmentID_perm (permissions:t) : bool := 
+    has_perm permissions CAP_PERM_COMPARTMENT_ID.
+  Definition has_branch_sealed_pair_perm (permissions:t) : bool := 
+    has_perm permissions CAP_PERM_BRANCH_SEALED_PAIR.
+  Definition has_ccall_perm (permissions:t) : bool := 
+    has_branch_sealed_pair_perm permissions.
+  Definition has_mutable_load_perm (permissions:t) : bool := 
+    has_perm permissions CAP_PERM_MUTABLE_LOAD.
+          
+  Definition get_user_perms (permissions:t) : list bool := 
+    [ has_user1_perm permissions; has_user2_perm permissions; 
+      has_user3_perm permissions; has_user4_perm permissions ]. 
+
+  Definition make_permissions (perms: list perm) : list bool :=  
+    let isLoad_perm : (perm -> bool) := fun p => match p with Load_perm => true | _ => false end in 
+    let isStore_perm : (perm -> bool) := fun p => match p with Store_perm => true | _ => false end in 
+    let isExecute_perm : (perm -> bool) := fun p => match p with Execute_perm => true | _ => false end in 
+    let isLoadCap_perm : (perm -> bool) := fun p => match p with LoadCap_perm => true | _ => false end in 
+    let isStoreCap_perm : (perm -> bool) := fun p => match p with StoreCap_perm => true | _ => false end in 
+    let isStoreLocalCap_perm : (perm -> bool) := fun p => match p with StoreLocalCap_perm => true | _ => false end in 
+    let isSeal_perm : (perm -> bool) := fun p => match p with Seal_perm => true | _ => false end in 
+    let isUnseal_perm : (perm -> bool) := fun p => match p with Unseal_perm => true | _ => false end in 
+    let isSystem_perm : (perm -> bool) := fun p => match p with System_perm => true | _ => false end in 
+    let isBranchSealedPair_perm : (perm -> bool) := fun p => match p with BranchSealedPair_perm => true | _ => false end in 
+    let isCompartmentID_perm : (perm -> bool) := fun p => match p with CompartmentID_perm => true | _ => false end in 
+    let isMutableLoad_perm : (perm -> bool) := fun p => match p with MutableLoad_perm => true | _ => false end in 
+    let isUser1_perm : (perm -> bool) := fun p => match p with User1_perm => true | _ => false end in 
+    let isUser2_perm : (perm -> bool) := fun p => match p with User2_perm => true | _ => false end in 
+    let isUser3_perm : (perm -> bool) := fun p => match p with User3_perm => true | _ => false end in 
+    let isUser4_perm : (perm -> bool) := fun p => match p with User4_perm => true | _ => false end in 
+    let isExecutive_perm : (perm -> bool) := fun p => match p with Executive_perm => true | _ => false end in 
+    let isGlobal_perm : (perm -> bool) := fun p => match p with Global_perm => true | _ => false end in 
+      [ existsb (isGlobal_perm) perms;           existsb (isExecutive_perm) perms; 
+        existsb (isUser1_perm) perms;            existsb (isUser2_perm) perms;  
+        existsb (isUser3_perm) perms;            existsb (isUser4_perm) perms;   
+        existsb (isMutableLoad_perm) perms;      existsb (isCompartmentID_perm) perms; 
+        existsb (isBranchSealedPair_perm) perms; existsb (isSystem_perm) perms;    
+        existsb (isUnseal_perm) perms;           existsb (isSeal_perm) perms;     
+        existsb (isStoreLocalCap_perm) perms;    existsb (isStoreCap_perm) perms; 
+        existsb (isLoadCap_perm) perms;          existsb (isExecute_perm) perms;  
+        existsb (isStore_perm) perms;            existsb (isLoad_perm) perms  ].
+
+  Program Definition perm_and_user_perms (perms:t) (user_perms:list bool) : t := 
+    let user_perm_4 := (nth 3 user_perms false) && (has_user4_perm perms) in   
+    let user_perm_3 := (nth 2 user_perms false) && (has_user3_perm perms) in 
+    let user_perm_2 := (nth 1 user_perms false) && (has_user2_perm perms) in 
+    let user_perm_1 := (nth 0 user_perms false) && (has_user1_perm perms) in 
+    @of_list_bool [ has_global_perm perms; has_executive_perm perms; 
+    user_perm_1; user_perm_2; user_perm_3; user_perm_4; has_mutable_load_perm perms;
+    has_compartmentID_perm perms; has_branch_sealed_pair_perm perms; has_system_access_perm perms;
+    has_unseal_perm perms; has_seal_perm perms; has_store_local_cap_perm perms; has_store_cap_perm perms;
+    has_load_cap_perm perms; has_execute_perm perms; has_store_perm perms; has_load_perm perms ] _.
+   Next Obligation. reflexivity. Defined.
+      
+  Program Definition perm_p0 : t := 
+    @of_list_bool (make_permissions []) _.
+   Next Obligation. reflexivity. Defined.
+
+  Program Definition perm_Universal : t := 
+    @of_list_bool (make_permissions [ Global_perm; Executive_perm; User1_perm; User2_perm; 
+    User3_perm; User4_perm; MutableLoad_perm; CompartmentID_perm; BranchSealedPair_perm; 
+    System_perm; Unseal_perm; Seal_perm; StoreLocalCap_perm; StoreCap_perm; LoadCap_perm; 
+    Execute_perm; Store_perm; Load_perm ]) _.
+    Next Obligation. reflexivity. Defined.
+
+  Program Definition perm_alloc : t :=
+    @of_list_bool (make_permissions [ Load_perm; Store_perm; LoadCap_perm; StoreCap_perm; StoreLocalCap_perm ]) _.
+    Next Obligation. reflexivity. Defined.
+
+  Program Definition perm_alloc_fun : t := 
+    @of_list_bool (make_permissions [ Load_perm; Execute_perm; LoadCap_perm ]) _.
+    Next Obligation. reflexivity. Defined.
+
+  Program Definition perm_clear_global (perms:t) : t :=
+    @of_list_bool [ false; has_executive_perm perms; has_user1_perm perms; has_user2_perm perms; has_user3_perm perms; has_user4_perm perms; 
+    has_mutable_load_perm perms; has_compartmentID_perm perms; has_branch_sealed_pair_perm perms; has_system_access_perm perms; has_unseal_perm perms;
+    has_seal_perm perms; has_store_local_cap_perm perms; has_store_cap_perm perms; has_load_cap_perm perms; has_execute_perm perms; has_store_perm perms;
+    has_load_perm perms ] _.
+    Next Obligation. reflexivity. Defined.
+
+  Program Definition perm_clear_executive (perms:t) : t :=
+    @of_list_bool [ has_global_perm perms; false; has_user1_perm perms; has_user2_perm perms; has_user3_perm perms; has_user4_perm perms;
+    has_mutable_load_perm perms; has_compartmentID_perm perms; has_branch_sealed_pair_perm perms; has_system_access_perm perms; has_unseal_perm perms;
+    has_seal_perm perms; has_store_local_cap_perm perms; has_store_cap_perm perms; has_load_cap_perm perms; has_execute_perm perms; has_store_perm perms;
+    has_load_perm perms ] _.
+    Next Obligation. reflexivity. Defined.
+    
+  Program Definition perm_clear_execute (perms:t) : t :=
+   @of_list_bool [ has_global_perm perms; has_executive_perm perms; has_user1_perm perms; has_user2_perm perms; has_user3_perm perms; has_user4_perm perms; 
+   has_mutable_load_perm perms; has_compartmentID_perm perms; has_branch_sealed_pair_perm perms; has_system_access_perm perms; has_unseal_perm perms;
+   has_seal_perm perms; has_store_local_cap_perm perms; has_store_cap_perm perms; has_load_cap_perm perms; false; has_store_perm perms;
+   has_load_perm perms ] _.
+   Next Obligation. reflexivity. Defined.
+ 
+  Program Definition perm_clear_load (perms:t) : t :=
+    @of_list_bool [ has_global_perm perms; has_executive_perm perms; has_user1_perm perms; has_user2_perm perms; has_user3_perm perms; has_user4_perm perms; 
+    has_mutable_load_perm perms; has_compartmentID_perm perms; has_branch_sealed_pair_perm perms; has_system_access_perm perms; has_unseal_perm perms;
+    has_seal_perm perms; has_store_local_cap_perm perms; has_store_cap_perm perms; has_load_cap_perm perms; has_execute_perm perms; has_store_perm perms;
+    false ] _.
+    Next Obligation. reflexivity. Defined.
+  
+  Program Definition perm_clear_load_cap (perms:t) : t :=
+    @of_list_bool [ has_global_perm perms; has_executive_perm perms; has_user1_perm perms; has_user2_perm perms; has_user3_perm perms; has_user4_perm perms; 
+    has_mutable_load_perm perms; has_compartmentID_perm perms; has_branch_sealed_pair_perm perms; has_system_access_perm perms; has_unseal_perm perms;
+    has_seal_perm perms; has_store_local_cap_perm perms; has_store_cap_perm perms; false; has_execute_perm perms; has_store_perm perms;
+    has_load_perm perms ] _.
+    Next Obligation. reflexivity. Defined.
+  
+  Program Definition perm_clear_seal (perms:t) : t :=
+    @of_list_bool [ has_global_perm perms; has_executive_perm perms; has_user1_perm perms; has_user2_perm perms; has_user3_perm perms; has_user4_perm perms; 
+    has_mutable_load_perm perms; has_compartmentID_perm perms; has_branch_sealed_pair_perm perms; has_system_access_perm perms; has_unseal_perm perms;
+    false; has_store_local_cap_perm perms; has_store_cap_perm perms; has_load_cap_perm perms; has_execute_perm perms; has_store_perm perms;
+    has_load_perm perms ] _.
+    Next Obligation. reflexivity. Defined.
+  
+  Program Definition perm_clear_store (perms:t) : t :=
+    @of_list_bool [ has_global_perm perms; has_executive_perm perms; has_user1_perm perms; has_user2_perm perms; has_user3_perm perms; has_user4_perm perms; 
+    has_mutable_load_perm perms; has_compartmentID_perm perms; has_branch_sealed_pair_perm perms; has_system_access_perm perms; has_unseal_perm perms;
+    has_seal_perm perms; has_store_local_cap_perm perms; has_store_cap_perm perms; has_load_cap_perm perms; has_execute_perm perms; false;
+    has_load_perm perms ] _.
+    Next Obligation. reflexivity. Defined.  
+
+  Program Definition perm_clear_store_cap (perms:t) : t :=
+    @of_list_bool [ has_global_perm perms; has_executive_perm perms; has_user1_perm perms; has_user2_perm perms; has_user3_perm perms; has_user4_perm perms; 
+    has_mutable_load_perm perms; has_compartmentID_perm perms; has_branch_sealed_pair_perm perms; has_system_access_perm perms; has_unseal_perm perms;
+    has_seal_perm perms; has_store_local_cap_perm perms; false; has_load_cap_perm perms; has_execute_perm perms; has_store_perm perms;
+    has_load_perm perms ] _.
+    Next Obligation. reflexivity. Defined.
+
+  Program Definition perm_clear_store_local_cap (perms:t) : t :=
+    @of_list_bool [ has_global_perm perms; has_executive_perm perms; has_user1_perm perms; has_user2_perm perms; has_user3_perm perms; has_user4_perm perms; 
+    has_mutable_load_perm perms; has_compartmentID_perm perms; has_branch_sealed_pair_perm perms; has_system_access_perm perms; has_unseal_perm perms;
+    has_seal_perm perms; false; has_store_cap_perm perms; has_load_cap_perm perms; has_execute_perm perms; has_store_perm perms;
+    has_load_perm perms ] _.
+    Next Obligation. reflexivity. Defined.
+
+  Program Definition perm_clear_system_access (perms:t) : t :=
+    @of_list_bool [ has_global_perm perms; has_executive_perm perms; has_user1_perm perms; has_user2_perm perms; has_user3_perm perms; has_user4_perm perms; 
+    has_mutable_load_perm perms; has_compartmentID_perm perms; has_branch_sealed_pair_perm perms; false; has_unseal_perm perms;
+    has_seal_perm perms; has_store_local_cap_perm perms; has_store_cap_perm perms; has_load_cap_perm perms; has_execute_perm perms; has_store_perm perms;
+    has_load_perm perms ] _.
+    Next Obligation. reflexivity. Defined.
+
+  Program Definition perm_clear_unseal (perms:t) : t :=
+    @of_list_bool [ has_global_perm perms; has_executive_perm perms; has_user1_perm perms; has_user2_perm perms; has_user3_perm perms; has_user4_perm perms; 
+    has_mutable_load_perm perms; has_compartmentID_perm perms; has_branch_sealed_pair_perm perms; has_system_access_perm perms; false;
+    has_seal_perm perms; has_store_local_cap_perm perms; has_store_cap_perm perms; has_load_cap_perm perms; has_execute_perm perms; has_store_perm perms;
+    has_load_perm perms ] _.
+    Next Obligation. reflexivity. Defined.
+
+  Program Definition perm_clear_branch_sealed_pair (perms:t) : t :=
+    @of_list_bool [ has_global_perm perms; has_executive_perm perms; has_user1_perm perms; has_user2_perm perms; has_user3_perm perms; has_user4_perm perms; 
+    has_mutable_load_perm perms; has_compartmentID_perm perms; false; has_system_access_perm perms; has_unseal_perm perms;
+    has_seal_perm perms; has_store_local_cap_perm perms; has_store_cap_perm perms; has_load_cap_perm perms; has_execute_perm perms; has_store_perm perms;
+    has_load_perm perms ] _.
+    Next Obligation. reflexivity. Defined.
+  Program Definition perm_clear_ccall (perms:t) : t := 
+    perm_clear_branch_sealed_pair perms.  
+  Program Definition perm_clear_mutable_load (perms:t) : t :=
+    @of_list_bool [ has_global_perm perms; has_executive_perm perms; has_user1_perm perms; has_user2_perm perms; has_user3_perm perms; has_user4_perm perms; 
+    false; has_compartmentID_perm perms; has_branch_sealed_pair_perm perms; has_system_access_perm perms; has_unseal_perm perms;
+    has_seal_perm perms; has_store_local_cap_perm perms; has_store_cap_perm perms; has_load_cap_perm perms; has_execute_perm perms; has_store_perm perms;
+    has_load_perm perms ] _.
+    Next Obligation. reflexivity. Defined.  
+
+  Program Definition perm_clear_compartment_ID (perms:t) : t :=
+    @of_list_bool [ has_global_perm perms; has_executive_perm perms; has_user1_perm perms; has_user2_perm perms; has_user3_perm perms; has_user4_perm perms; 
+    has_mutable_load_perm perms; false; has_branch_sealed_pair_perm perms; has_system_access_perm perms; has_unseal_perm perms;
+    has_seal_perm perms; has_store_local_cap_perm perms; has_store_cap_perm perms; has_load_cap_perm perms; has_execute_perm perms; has_store_perm perms;
+    has_load_perm perms ] _.
+    Next Obligation. reflexivity. Defined.  
+
+  Program Definition perm_clear_user1 (perms:t) : t :=
+    @of_list_bool [ has_global_perm perms; has_executive_perm perms; false; has_user2_perm perms; has_user3_perm perms; has_user4_perm perms;  
+    has_mutable_load_perm perms; has_compartmentID_perm perms; has_branch_sealed_pair_perm perms; has_system_access_perm perms; has_unseal_perm perms;
+    has_seal_perm perms; has_store_local_cap_perm perms; has_store_cap_perm perms; has_load_cap_perm perms; has_execute_perm perms; has_store_perm perms;
+    has_load_perm perms ] _.
+    Next Obligation. reflexivity. Defined.    
+
+  Program Definition perm_clear_user2 (perms:t) : t :=
+    @of_list_bool [ has_global_perm perms; has_executive_perm perms; has_user1_perm perms; false; has_user3_perm perms; has_user4_perm perms;
+    has_mutable_load_perm perms; has_compartmentID_perm perms; has_branch_sealed_pair_perm perms; has_system_access_perm perms; has_unseal_perm perms;
+    has_seal_perm perms; has_store_local_cap_perm perms; has_store_cap_perm perms; has_load_cap_perm perms; has_execute_perm perms; has_store_perm perms;
+    has_load_perm perms ] _.
+    Next Obligation. reflexivity. Defined.  
+
+  Program Definition perm_clear_user3 (perms:t) : t :=
+    @of_list_bool [ has_global_perm perms; has_executive_perm perms; has_user1_perm perms; has_user2_perm perms; false; has_user4_perm perms; 
+    has_mutable_load_perm perms; has_compartmentID_perm perms; has_branch_sealed_pair_perm perms; has_system_access_perm perms; has_unseal_perm perms;
+    has_seal_perm perms; has_store_local_cap_perm perms; has_store_cap_perm perms; has_load_cap_perm perms; has_execute_perm perms; has_store_perm perms;
+    has_load_perm perms ] _.
+    Next Obligation. reflexivity. Defined.  
+
+  Program Definition perm_clear_user4 (perms:t) : t :=
+    @of_list_bool [ has_global_perm perms; has_executive_perm perms; has_user1_perm perms; has_user2_perm perms; has_user3_perm perms; false;
+    has_mutable_load_perm perms; has_compartmentID_perm perms; has_branch_sealed_pair_perm perms; has_system_access_perm perms; has_unseal_perm perms;
+    has_seal_perm perms; has_store_local_cap_perm perms; has_store_cap_perm perms; has_load_cap_perm perms; has_execute_perm perms; has_store_perm perms;
+    has_load_perm perms ] _.
+    Next Obligation. reflexivity. Defined.  
+  
+  Definition to_string (perms:t) : string :=
+    String.hex_string_of_int (bv_to_Z_unsigned perms).
+
+  Definition to_raw (perms:t) : Z := bv_to_Z_unsigned perms.
+
+  Definition of_list (l : list bool) : option t := 
+    if ((List.length l) =? (N_to_nat len))%nat then
+      Some (@mword_to_bv (Z.of_N len) (of_bools (List.rev l))) 
+    else None.
+  
+  Definition to_list (perms:t) : list bool := 
+    bv_to_list_bool perms.
+  
+End Permissions.
+
+
+
+Module Value <: VADDR.
+  Definition len:N := 64.
+  Definition t := bv len.
+
+  Definition of_Z (z:Z) : t := Z_to_bv len z.
+  Definition to_Z (v:t) : Z := bv_to_Z_unsigned v.
+
+  Definition bitwise_complement (a:Z) : Z :=
+    let bits := Z_to_binary (N_to_nat len) a in
     let bits := Vector.map negb bits in
     binary_value _ bits.
 
-  Definition eqb := Z.eqb.
-  Definition ltb := Z.ltb.
-  Definition leb := Z.leb.
-  Definition ltb_irref := Z.ltb_irrefl.
+  Definition eqb (v1:t) (v2:t) : bool := v1 =? v2.
+  Definition ltb (v1:t) (v2:t) : bool := v1 <? v2.
+  Definition leb (v1:t) (v2:t) : bool := v1 <=? v2.
+  
+  Definition ltb_irref: forall a:t, ltb a a = false.
+  Proof. intros. unfold ltb. unfold lt. rewrite Z.ltb_irrefl. reflexivity. Qed. 
+  
+End Value.
 
-End MorelloAddr.
 
-Module MoreloOTYPE <: OTYPE.
-  Definition t := Z.
-End MoreloOTYPE.
+Module ObjType <: OTYPE.
+  Definition len:N := 64.
+  Definition t := bv len.  (* ObtTypes are effectively 15-bit values,
+  but the ASL extracts this field from a cap as a 64-bit word, 
+  possibly to match the size of the objTypes stored in sealing caps *)
 
-Module MorelloCAP_SEAL_T <: CAP_SEAL_T.
+  (* Definition CAP_OTYPE_LO_BIT:N := 95.
+  Definition CAP_OTYPE_HI_BIT:N := 109.
+  Definition CAP_OTYPE_NUM_BITS:N := 15. *)
+  Definition CAP_MAX_OBJECT_TYPE:N := 32767.
+
+  Definition of_Z (z:Z) : t := Z_to_bv len z.
+  Definition to_Z (o:t) : Z := bv_to_Z_unsigned o.
+End ObjType.
+
+
+Module SealType <: CAP_SEAL_T. 
   Inductive cap_seal_t :=
   | Cap_Unsealed
   | Cap_SEntry (* "RB" in Morello *)
   | Cap_Indirect_SEntry (* "LB" in Morello *)
-  (* | Cap_Indirect_SEntry_Pair *) (* "LBP" in Morello. TODO see why unused *)
-  | Cap_Sealed (seal:MoreloOTYPE.t).
+  | Cap_Indirect_SEntry_Pair (* "LPB" in Morello. TODO see why unused *)
+  | Cap_Sealed (seal : ObjType.t).
+  
+  Definition t := cap_seal_t. 
 
-  Definition t := cap_seal_t.
-End MorelloCAP_SEAL_T.
-
-Module MorelloVADDR_INTERVAL <: VADDR_INTERVAL(MorelloAddr).
-  Definition t := (MorelloAddr.t * MorelloAddr.t)%type.
-
-  Definition addresses_in_interval intr addr :=
-    let '(base,limit) := intr in
-    andb (MorelloAddr.leb base addr) (MorelloAddr.ltb addr limit).
-
-  Definition ltb (a b:t):= false. (* TODO *)
-End MorelloVADDR_INTERVAL.
-
-Module MorelloPermission <: Permission.
-
-  Record morello_perm_record  :=
-    {
-      global: bool;
-      executive: bool ;
-
-      permits_load: bool;
-      permits_store: bool;
-      permits_execute: bool ;
-      permits_load_cap: bool;
-      permits_store_cap: bool;
-      permits_store_local_cap: bool;
-      permits_seal: bool;
-      permits_unseal: bool;
-      permits_system_access: bool;
-
-      permits_ccall: bool; (* called "permoit_branch_sealer_pair" in Morello *)
-
-      permit_compartment_id: bool; (* Morello-spefic? *)
-      permit_mutable_load : bool; (* Morello-spefic? *)
-
-      (* User[N] *)
-      user_perms: list bool;
-    }.
-
-
-  Definition t := morello_perm_record.
-
-  Definition user_perms_len := 4%nat.
-
-  (* convenience constant to be used as size in `mword` *)
-  Definition perms_zlen := Z.add (Z.of_nat user_perms_len) 14.
-
-  Definition perm_is_global := global.
-  Definition perm_is_execute := executive.
-  Definition perm_is_ccall := permits_ccall.
-  Definition perm_is_load := permits_load.
-  Definition perm_is_load_cap := permits_load_cap.
-  Definition perm_is_seal := permits_seal.
-  Definition perm_is_store := permits_store.
-  Definition perm_is_store_cap := permits_store_cap.
-  Definition perm_is_store_local_cap := permits_store_local_cap.
-  Definition perm_is_system_access := permits_system_access.
-  Definition perm_is_unseal := permits_unseal.
-
-  Definition get_user_perms := user_perms.
-
-  Definition TODO_ID (x:t) := x.
-
-  Definition perm_clear_global := TODO_ID.
-  Definition perm_clear_execute := TODO_ID.
-  Definition perm_clear_ccall := TODO_ID.
-  Definition perm_clear_load := TODO_ID.
-  Definition perm_clear_load_cap := TODO_ID.
-  Definition perm_clear_seal := TODO_ID.
-  Definition perm_clear_store := TODO_ID.
-  Definition perm_clear_store_cap := TODO_ID.
-  Definition perm_clear_store_local_cap := TODO_ID.
-  Definition perm_clear_system_access := TODO_ID.
-  Definition perm_clear_unseal := TODO_ID.
-
-  Definition perm_and_user_perms (p:t) (np:list bool):= p. (* TODO *)
-
-  Definition perm_p0:t :=
-    {|
-      global := false ;
-      executive := false ;
-      permits_load := false ;
-      permits_store := false ;
-      permits_execute := false ;
-      permits_load_cap := false ;
-      permits_store_cap := false ;
-      permits_store_local_cap := false ;
-      permits_seal := false ;
-      permits_unseal := false ;
-      permits_system_access := false ;
-      permits_ccall := false ;
-      permit_compartment_id := false ;
-      permit_mutable_load := false ;
-      user_perms := List.repeat false user_perms_len
-    |}.
-
-  Definition perm_alloc:t :=
-    {|
-      global := false ;
-      executive := false ;
-      permits_load := true ;
-      permits_store := true ;
-      permits_execute := false ;
-      permits_load_cap := true ;
-      permits_store_cap := true ;
-      permits_store_local_cap := true ;
-      permits_seal := false ;
-      permits_unseal := false ;
-      permits_system_access := false ;
-      permits_ccall := false ;
-      permit_compartment_id := false ;
-      permit_mutable_load := false ;
-      user_perms := List.repeat false user_perms_len
-    |}.
-
-  Definition perm_alloc_fun:t :=
-    {|
-      global := false ;
-      executive := false ;
-      permits_load := true ;
-      permits_store := false ;
-      permits_execute := true ;
-      permits_load_cap := true ;
-      permits_store_cap := false ;
-      permits_store_local_cap := false ;
-      permits_seal := false ;
-      permits_unseal := false ;
-      permits_system_access := false ;
-      permits_ccall := false ;
-      permit_compartment_id := false ;
-      permit_mutable_load := false ;
-      user_perms := List.repeat false user_perms_len
-    |}.
-
-  Definition to_string (p:t) := "TODO"%string.
-
-  (* raw permissoins in numeric format *)
-  Definition to_raw (p:t) := Z0. (*  TODO *)
-
-  Definition of_list (l: list bool): option t := None. (* TODO *)
-
-  Definition to_list (p_value : t) : list bool :=
-    List.app [ p_value.(global); p_value.(executive) ]
-      (List.app p_value.(user_perms)
-        [
-          p_value.(permit_mutable_load);
-          p_value.(permit_compartment_id);
-          p_value.(permits_ccall);
-          p_value.(permits_system_access);
-          p_value.(permits_unseal);
-          p_value.(permits_seal);
-          p_value.(permits_store_local_cap);
-          p_value.(permits_store_cap);
-          p_value.(permits_load_cap);
-          p_value.(permits_execute);
-          p_value.(permits_store);
-          p_value.(permits_load)
-        ]).
-
-End MorelloPermission.
-
-
-Module MorelloCapability <:
-  Capability
-    (MorelloAddr)
-  (MoreloOTYPE)
-  (MorelloCAP_SEAL_T)
-  (MorelloVADDR_INTERVAL)
-  (MorelloPermission).
-
-  Inductive morello_cap_t :=
-    {
-      valid : bool;
-      value : MorelloAddr.t;
-      obj_type : MoreloOTYPE.t;
-      bounds : MorelloVADDR_INTERVAL.t;
-      flags : list bool;
-      perms : MorelloPermission.t
-    }.
-
-  Definition with_valid valid (r : morello_cap_t) :=
-    Build_morello_cap_t valid r.(value) r.(obj_type) r.(bounds) r.(flags) r.(perms).
-  Definition with_value value (r : morello_cap_t) :=
-    Build_morello_cap_t r.(valid) value r.(obj_type) r.(bounds) r.(flags) r.(perms).
-  Definition with_obj_type obj_type (r : morello_cap_t) :=
-    Build_morello_cap_t r.(valid) r.(value) obj_type r.(bounds) r.(flags) r.(perms).
-  Definition with_bounds bounds (r : morello_cap_t) :=
-    Build_morello_cap_t r.(valid) r.(value) r.(obj_type) bounds r.(flags) r.(perms).
-  Definition with_flags flags (r : morello_cap_t) :=
-    Build_morello_cap_t r.(valid) r.(value) r.(obj_type) r.(bounds) flags r.(perms).
-  Definition with_perms perms (r : morello_cap_t) :=
-    Build_morello_cap_t r.(valid) r.(value) r.(obj_type) r.(bounds) r.(flags) perms.
-
-  Definition t := morello_cap_t.
-
-  Definition sizeof_vaddr : nat := MorelloAddr.sizeof_vaddr.
-
-  Definition vaddr_bits : nat := MorelloAddr.vaddr_bits.
-
-  Definition min_vaddr : Z := 0.
-
-  Definition max_vaddr : Z := Z.sub (Z.pow 2 (Z.of_nat vaddr_bits)) 1.
-
-  Definition cap_flags_len : nat := 8%nat.
-
-  Definition cap_is_valid (c_value : t) : bool := c_value.(valid).
-
-  Definition cap_get_obj_type (c_value : t)  := c_value.(obj_type).
-
-  Definition cap_get_value (c_value : t)  := c_value.(value).
-
-  Definition cap_get_bounds (c_value : t) := c_value.(bounds).
-
-  Definition cap_get_offset (c_value : t) : Z :=
-    Z.sub c_value.(value) (fst c_value.(bounds)).
-
-  Definition cap_SEAL_TYPE_UNSEALED := 0.
-  Definition cap_SEAL_TYPE_RB  := 1.
-  Definition cap_SEAL_TYPE_LPB := 2.
-  Definition cap_SEAL_TYPE_LB  := 3.
-
-  Definition cap_get_seal (c_value : t) : MorelloCAP_SEAL_T.t :=
-    let x_value := c_value.(obj_type) in
-    if Z.eqb x_value cap_SEAL_TYPE_UNSEALED then
-      MorelloCAP_SEAL_T.Cap_Unsealed
-    else
-      if Z.eqb x_value cap_SEAL_TYPE_RB then
-        MorelloCAP_SEAL_T.Cap_SEntry
-      else
-        if Z.eqb x_value cap_SEAL_TYPE_LPB then
-          MorelloCAP_SEAL_T.Cap_Indirect_SEntry
-        else
-          if Z.eqb x_value cap_SEAL_TYPE_LB then
-            MorelloCAP_SEAL_T.Cap_Indirect_SEntry
-          else
-            MorelloCAP_SEAL_T.Cap_Sealed x_value.
-
-  Definition cap_get_flags (c_value : t) : list bool := c_value.(flags).
-
-  Definition cap_get_perms c_value := c_value.(perms).
-
-  (* helper function to convert [mword] to list of booleans *)
-  Definition mword_to_bools {n:Z} (w: mword n) :=
-    List.map bool_of_bit (bits_of w).
-
-  Definition flags_from_value_bits (x : mword 64) : list bool :=
-    let x := zero_extend x 64 in
-    let xl := mword_to_bools x in
-    List.skipn (Nat.sub 64 8)%nat xl.
-
-  Definition flags_from_value (v : MorelloAddr.t) : list bool :=
-    let w := mword_of_int v (len:= Z.of_nat vaddr_bits) in
-    flags_from_value_bits w.
-
-  Definition decode_word (bits : mword 129) : option t :=
-    let value' := CapGetValue bits in
-    let value := projT1 (uint value') in
-    let '(base', limit', isExponentValid) := CapGetBounds bits in
-    if negb isExponentValid
-    then None
-    else
-      let flags := flags_from_value_bits value' in
-      let perms' := CapGetPermissions bits in
-      let perms_data := mword_to_bools perms' in
-      match MorelloPermission.of_list perms_data with
-      | None => None
-      | Some perms =>
-          let otype := projT1 (uint (CapGetObjectType bits)) in
-          Some
-            {| valid := CapIsTagSet bits;
-              value := value;
-              obj_type := otype;
-              bounds := (projT1 (uint base'), projT1 (uint limit'));
-              flags := flags;
-              perms := perms |}
-      end.
-
-  Program Definition decode (bytes : list ascii) (tag : bool) : option t :=
-    if Nat.eqb (List.length bytes) 16%nat then
-      let bytes := List.rev bytes in
-      let bits := tag::(bool_bits_of_bytes bytes) in
-      let bitsu := List.map bitU_of_bool bits in
-      let w := vec_of_bits bitsu in
-      decode_word w
-    else
-      None.
-  Next Obligation.
-    admit. (* TODO: prove that (lenght (bool_bits_of_bytes)==128)
-              and ehence [w] is 129-bit long *)
-  Admitted.
-
-  Definition cap_c0 (_: unit) : t :=
-    {| valid := false;
-      value := 0;
-      obj_type := 0;
-      bounds := (0, 18446744073709551616);
-      flags := [false; false; false; false; false; false; false; false];
-      perms :=
-        {|
-          MorelloPermission.global := false;
-          MorelloPermission.executive := false ;
-          MorelloPermission.permits_load := false;
-          MorelloPermission.permits_store := false;
-          MorelloPermission.permits_execute := false ;
-          MorelloPermission.permits_load_cap := false;
-          MorelloPermission.permits_store_cap := false;
-          MorelloPermission.permits_store_local_cap := false;
-          MorelloPermission.permits_seal := false;
-          MorelloPermission.permits_unseal := false;
-          MorelloPermission.permits_system_access := false;
-          MorelloPermission.permits_ccall := false;
-          MorelloPermission.permit_compartment_id := false;
-          MorelloPermission.permit_mutable_load := false;
-
-          MorelloPermission.user_perms := [false; false; false; false]
-        |}
-    |}.
-
-  Definition alloc_cap (a_value : MorelloAddr.t) (size : Z) : t :=
-    {|
-      valid := true;
-      value := a_value;
-      obj_type := cap_SEAL_TYPE_UNSEALED;
-      bounds := (a_value, (Z.add a_value size));
-      flags := flags_from_value a_value;
-      perms := MorelloPermission.perm_alloc
-    |}.
-
-  Definition alloc_fun (a_value : MorelloAddr.t) : t :=
-    {|
-      valid := true;
-      value := a_value;
-      obj_type := cap_SEAL_TYPE_RB;
-      bounds := (a_value, (Z.succ (Z.succ a_value)));
-      flags := flags_from_value a_value;
-      perms := MorelloPermission.perm_alloc_fun
-    |}.
-
-  Definition vaddr_in_range (a_value : Z) : bool :=
-    Z.geb a_value min_vaddr && Z.leb a_value max_vaddr.
-
-  Definition CapSetPermissins
-    (zc: mword 129)
-    (zp: mword MorelloPermission.perms_zlen)
-    : mword 129
-    :=
-    update_subrange_vec_dec zc CAP_PERMS_HI_BIT CAP_PERMS_LO_BIT zp.
-
-  Program Definition encode_to_word (isexact : bool) (c : t) : mword 129 :=
-    let bits := CapNull tt in
-    let bits :=
-      CapSetTag bits
-        (mword_of_int (len:=64) (if cap_is_valid c then 1 else 0))
-    in
-    let bits :=
-      CapSetObjectType
-        bits (mword_of_int (len:=64) (cap_get_obj_type c)) in
-    let '(base, limit) := cap_get_bounds c in
-    let len := Z.sub limit base in
-    let bits := CapSetValue bits (mword_of_int (len:=64) base) in
-    let bits := CapSetBounds bits (mword_of_int (len:=65) len) isexact in
-    let bits := CapSetValue bits (mword_of_int (len:=64) (cap_get_value c)) in
-    let flags := List.map bitU_of_bool (cap_get_flags c) in
-    let flags := vec_of_bits flags in
-    let flags := zero_extend flags 64 in
-    let bits := CapSetFlags bits flags in
-    let perms :=
-      List.map bitU_of_bool (MorelloPermission.to_list (cap_get_perms c)) in
-    let perms := vec_of_bits perms in
-    let bits := CapSetPermissins bits perms in
-    bits.
-  Next Obligation.
-    (* TODO: prove that [(MorelloPermission.to_list (cap_get_perms c)) = perms_len] *)
-  Admitted.
-
-  Definition cap_vaddr_representable (c : t) (a : Z) : bool
-    :=
-    vaddr_in_range a &&
-      CapIsRepresentable (encode_to_word true c) (mword_of_int (len:=64) a).
-
-  Definition cap_bounds_representable_exactly
-    (c : t) (intr : MorelloVADDR_INTERVAL.t) : bool
-    :=
-    let '(base, limit) := intr in
-    let bits := encode_to_word true c in
-    let len := Z.sub limit base in
-    let base' := mword_of_int (len:=64) base in
-    let len' := mword_of_int (len:=65) len in
-    let bits := CapSetValue bits base' in
-    let bits := CapSetBounds bits len' true in
-    CapIsTagSet bits.
-
-  Definition cap_invalidate (c : t) : t := with_valid false c.
-
-  Definition is_sealed (c : t) : bool :=
-    match cap_get_seal c with
-    | MorelloCAP_SEAL_T.Cap_Unsealed => false
-    | _ => true
+  Definition get_seal_ot (seal:t) : ObjType.t :=
+    match seal with 
+      Cap_Unsealed => ObjType.of_Z 0
+    | Cap_SEntry => ObjType.of_Z 1
+    | Cap_Indirect_SEntry => ObjType.of_Z 3
+    | Cap_Indirect_SEntry_Pair => ObjType.of_Z 2
+    | Cap_Sealed seal => seal
     end.
 
-  Definition invalidate_if_sealded (c_value : t) : t :=
-    if is_sealed c_value then
-      cap_invalidate c_value
+  Definition sealed_entry_ot := get_seal_ot Cap_SEntry.
+  Definition sealed_indirect_entry_ot := get_seal_ot Cap_Indirect_SEntry.
+  Definition sealed_indirect_entry_pair_ot := get_seal_ot Cap_Indirect_SEntry_Pair.
+
+End SealType.
+
+
+Module Bounds <: VADDR_INTERVAL(Value).
+  (* Definition t := bv 87. *)
+  Definition bound_len:N := 65.
+  Definition t := ((bv bound_len) * (bv bound_len))%type.
+  Definition of_Zs (bounds : Z * Z) : t :=
+    let '(base,limit) := bounds in   
+    (Z_to_bv bound_len base, Z_to_bv bound_len limit). 
+  Definition to_Zs (bounds : t) : Z * Z :=
+    let (base,top) := bounds in   
+    (bv_to_Z_unsigned base, bv_to_Z_unsigned top).
+
+  Definition address_is_in_interval (bounds:Bounds.t) (value:Value.t) : bool :=
+    let '(base,limit) := bounds in 
+    let value : (bv Bounds.bound_len) := bv_to_bv value in 
+    (base <=? value) && (value <? limit).
+
+  (* Vadim: is this what we want? *)
+  Definition ltb (a b:t) := 
+    let '(base_a, limit_a) := a in
+    let '(base_b, limit_b) := b in
+    ((base_a <? base_b) && (limit_a <=? limit_b))
+    || ((base_a <=? base_b) && (limit_a <? limit_b)).
+
+End Bounds. 
+
+
+Module Cap <: Capability (Value) (ObjType) (SealType) (Bounds) (Permissions).
+  Definition len:N := 129.
+  Definition t := bv len.
+
+  Definition of_Z (z:Z) : t := Z_to_bv len z.
+     
+  Definition cap_SEAL_TYPE_UNSEALED : ObjType.t := ObjType.of_Z 0.
+  Definition cap_SEAL_TYPE_RB : ObjType.t := ObjType.of_Z 1. 
+  Definition cap_SEAL_TYPE_LPB : ObjType.t := ObjType.of_Z 2. 
+  Definition cap_SEAL_TYPE_LB : ObjType.t := ObjType.of_Z 3.
+
+  Definition sizeof_vaddr := 8%N. (* in bytes *)
+  (* Definition vaddr_bits := sizeof_vaddr * 8. *)
+  Definition min_vaddr := Z_to_bv (sizeof_vaddr*8) 0.  
+  Definition max_vaddr := Z_to_bv (sizeof_vaddr*8) (bv_modulus (sizeof_vaddr*8)).
+  
+  Definition cap_c0 (u:unit) : t := mword_to_bv (CapNull u).
+
+  Definition cap_cU (u:unit) : t := mword_to_bv (concat_vec (Ones 19) (Zeros 110)).
+
+  Definition bound_null (u:unit) : bv 65 := Z_to_bv 65 0.
+
+  Definition cap_flags_len := 8 % nat.
+  Definition Flags := { l : list bool | length l = cap_flags_len }.
+  
+  Definition cap_get_value (cap:t) : Value.t := 
+    mword_to_bv (CapGetValue (bv_to_mword cap)).
+  
+  Definition cap_get_obj_type (cap:t) : ObjType.t := 
+    mword_to_bv (CapGetObjectType (bv_to_mword cap)).
+
+  Definition cap_get_bounds (cap:t) : Bounds.t * bool :=
+    let '(base_mw, limit_mw, isExponentValid) := CapGetBounds (bv_to_mword cap) in
+    let base_bv := mword_to_bv base_mw in
+    let limit_bv := mword_to_bv limit_mw in 
+    ((base_bv, limit_bv), isExponentValid).
+
+  Definition cap_get_offset (cap:t) : Z :=
+    (mword_to_bv (CapGetOffset (bv_to_mword cap))).(bv_unsigned).
+        
+  Definition cap_get_seal (cap:t) : SealType.t := 
+    let ot:ObjType.t := cap_get_obj_type cap in
+    if (ot =? cap_SEAL_TYPE_UNSEALED)%stdpp then SealType.Cap_Unsealed else
+    if (ot =? cap_SEAL_TYPE_RB)%stdpp then SealType.Cap_SEntry else
+    if (ot =? cap_SEAL_TYPE_LPB)%stdpp then SealType.Cap_Indirect_SEntry else 
+    if (ot =? cap_SEAL_TYPE_LB)%stdpp then SealType.Cap_Indirect_SEntry else (* confirm duplication *)
+    SealType.Cap_Sealed ot.
+    
+  (* The flags are the top byte of the value. *)
+  Program Definition cap_get_flags (cap:t) : Flags := 
+    let m : (mword _) := subrange_vec_dec (bv_to_mword cap) CAP_VALUE_HI_BIT CAP_FLAGS_LO_BIT in
+    let l : (list bool) := (mword_to_list_bool m) in
+    exist _ l _.
+  Next Obligation. reflexivity. Defined.  
+
+  Definition cap_get_perms (cap:t) : Permissions.t := 
+    mword_to_bv (CapGetPermissions (bv_to_mword cap)).
+
+  Definition cap_is_sealed (cap:t) : bool :=
+    CapIsSealed (bv_to_mword cap).
+  
+  Definition cap_invalidate (cap:t) : t := mword_to_bv (CapWithTagClear (bv_to_mword cap)).
+  
+  Definition cap_set_value (cap:t) (value:Value.t) : t :=
+    let new_cap := mword_to_bv (CapSetValue (bv_to_mword cap) (bv_to_mword value)) in 
+    if (cap_is_sealed cap) then (cap_invalidate new_cap) else new_cap.
+  
+  Definition cap_set_flags (cap:t) (f:Flags) : t :=
+    let new_cap :=
+      let flags_m : (mword (Z.of_nat cap_flags_len)) := of_bools (proj1_sig f) in
+      let flags' : (mword 64) := concat_vec flags_m (Zeros (64 - (Z.of_nat cap_flags_len))) in 
+        mword_to_bv (CapSetFlags (bv_to_mword cap) flags')       in 
+    if (cap_is_sealed cap) then (cap_invalidate new_cap) else new_cap.
+   
+  Definition cap_set_objtype (cap:t) (ot:ObjType.t) : t :=
+    mword_to_bv (CapSetObjectType (bv_to_mword cap) (zero_extend (bv_to_mword ot) 64)).
+
+  (* [perms] must contain [1] for permissions to be cleared and [0] for those to be kept *)
+  Definition cap_narrow_perms (cap:t) (perms:Permissions.t) : t :=
+    let perms_mw : (mword (Z.of_N Permissions.len)) := bv_to_mword perms in 
+    let mask : (mword 64) := 
+      zero_extend perms_mw 64 in
+    let new_cap := mword_to_bv (CapClearPerms (bv_to_mword cap) mask) in 
+    if (cap_is_sealed cap) then (cap_invalidate new_cap) else new_cap.
+
+  Definition cap_clear_global_perm (cap:t) : t := 
+    cap_narrow_perms cap (list_bool_to_bv (Permissions.make_permissions [Permissions.Global_perm])).
+
+  Definition cap_set_bounds (cap : t) (bounds : Bounds.t) (exact : bool) : t :=
+    (* CapSetBounds sets the lower bound to the value of the input cap,
+       so we first have to set the value of cap to bounds.base. *)
+    let '(base,limit) := bounds in
+    let base_as_val : Value.t := bv_to_bv base in  
+    let new_cap := cap_set_value cap base_as_val in 
+    let req_len : (mword (Z.of_N Bounds.bound_len)) := 
+      mword_of_int (Z.sub (bv_to_Z_unsigned limit) (bv_to_Z_unsigned base)) in 
+    let new_cap := 
+      mword_to_bv (CapSetBounds (bv_to_mword new_cap) req_len exact) in 
+    if (cap_is_sealed cap) then (cap_invalidate new_cap) else new_cap.
+
+  Definition cap_narrow_bounds (cap : t) (bounds : Bounds.t) : t :=
+    cap_set_bounds cap bounds false.
+
+  Definition cap_narrow_bounds_exact (cap : t) (bounds : Bounds.t) : t :=
+    cap_set_bounds cap bounds true.
+
+  Definition cap_is_valid (cap:t) : bool := Bool.eqb (CapIsTagClear (bv_to_mword cap)) false.
+
+  Definition cap_is_invalid (cap:t) : bool := negb (cap_is_valid cap).
+    
+  Definition cap_is_unsealed (cap:t) : bool := negb (cap_is_sealed cap).
+  
+  Definition cap_is_in_bounds (cap:t) : bool := CapIsInBounds (bv_to_mword cap).
+
+  Definition cap_is_not_in_bounds (cap:t) : bool := negb (cap_is_in_bounds cap).  
+  
+  Definition cap_is_exponent_out_of_range (cap:t) : bool :=
+    CapIsExponentOutOfRange (bv_to_mword cap).
+
+  Definition cap_has_perm (cap:t) :=
+    let perms : (mword 64) := zero_extend (bv_to_mword (cap_get_perms cap)) 64 in 
+    fun perm => CapPermsInclude perms perm.
+
+  Definition cap_has_seal_perm (cap:t) : bool := cap_has_perm cap CAP_PERM_SEAL.
+
+  Definition cap_has_unseal_perm (cap:t) : bool := cap_has_perm cap CAP_PERM_UNSEAL.
+
+  Definition cap_has_global_perm (cap:t) : bool := cap_has_perm cap CAP_PERM_GLOBAL.
+
+  Definition cap_seal (c : t) (k : t) : t :=
+    let key : ObjType.t := (cap_get_value k) in 
+    let sealed_cap := cap_set_objtype c key in 
+    if (cap_is_valid c) && (cap_is_valid k) && 
+       (cap_is_unsealed c) && (cap_is_unsealed k) && 
+       (cap_has_seal_perm k) && (cap_is_in_bounds k) &&
+       (Z.to_N (bv_to_Z_unsigned key) <=? ObjType.CAP_MAX_OBJECT_TYPE)%N then 
+       sealed_cap
     else
-      c_value.
+       cap_invalidate sealed_cap.
 
-  Definition cap_set_value (c_value : t) (cv : MorelloAddr.t) : t :=
-    if cap_vaddr_representable c_value cv then
-      invalidate_if_sealded
-        (with_flags (flags_from_value cv) (with_value cv c_value))
+  Definition cap_unseal (sealed_cap:t) (unsealing_cap:t) : t :=
+    let value := cap_get_value unsealing_cap in 
+    let key := cap_get_obj_type sealed_cap in 
+    let unsealed_sealed_cap := mword_to_bv (CapUnseal (bv_to_mword sealed_cap)) in 
+    let unsealed_sealed_cap := 
+      if (negb (cap_has_global_perm unsealing_cap)) then
+        cap_clear_global_perm unsealed_sealed_cap
+      else unsealed_sealed_cap in 
+    if (cap_is_valid sealed_cap && cap_is_valid unsealing_cap 
+        && cap_is_sealed sealed_cap && cap_is_unsealed unsealing_cap
+        && cap_has_unseal_perm unsealing_cap
+        && cap_is_in_bounds unsealing_cap && (key =? value) ) then 
+      unsealed_sealed_cap
+    else 
+      cap_invalidate unsealed_sealed_cap.
+
+  Definition cap_seal_immediate (cap : t) (seal_ot : ObjType.t) 
+    `{ArithFact ((bv_to_Z_unsigned seal_ot >? 0)%Z && (bv_to_Z_unsigned seal_ot <=? 4)%Z)} : t :=
+    let new_cap := cap_set_objtype cap seal_ot in 
+    if (cap_is_valid cap && cap_is_unsealed cap) then 
+      new_cap
     else
-      cap_invalidate (with_value cv c_value).
+      cap_invalidate new_cap.
 
-  Definition cap_narrow_bounds (c : t) (bounds : Z * Z) : t :=
-    let '(a0, a1) := bounds in
-    (* TODO(CHERI): this is placeholder representation. Due to representability constraints bounds may not end up exact as passed *)
-    (* assert vaddr_in_range a0 && vaddr_in_range a1 *)
-    invalidate_if_sealded (with_bounds (a0, a1) c).
+  (* For sealing with RB *)
+  Definition cap_seal_entry (cap:t) : t := 
+    cap_seal_immediate cap SealType.sealed_entry_ot.
 
-  Definition cap_narrow_bounds_exact (c : t) (bounds : Z * Z)  : t :=
-    let '(a0, a1) := bounds in
-    (* assert vaddr_in_range a0 && vaddr_in_range a1 *)
-    invalidate_if_sealded c.
+  (* For sealing with LB *)
+  Definition cap_seal_indirect_entry (cap:t) : t := 
+    cap_seal_immediate cap SealType.sealed_indirect_entry_ot.
 
-  Definition cap_narrow_perms (c : t) (p : MorelloPermission.t) : t :=
-    let l0 := MorelloPermission.to_list c.(perms) in
-    let l1 := MorelloPermission.to_list p in
-    let l := List.map (fun '(a,b) =>  andb a b) (List.combine l0 l1) in
-    match MorelloPermission.of_list l with
-    | Some p => invalidate_if_sealded (with_perms p c)
-    | None => c (* impossible case *)
-    end.
+  (* For sealing with LPB *)  
+  Definition cap_seal_indirect_entry_pair (cap:t) : t := 
+    cap_seal_immediate cap SealType.sealed_indirect_entry_pair_ot.
 
-  Definition cap_seal (c : t) (k : t) : t := cap_set_value c (cap_get_value k).
+  (* Confirm the type of the function is ok *)  
+  Definition representable_alignment_mask (len:N) : N :=
+    mword_to_N (CapGetRepresentableMask (@mword_of_int (Z.of_N Value.len) (Z.of_N len))).
 
-  Definition cap_seal_entry (c : t) : t := c. (* TODO: looks like it is not implemented yet *)
+  (* Will need to see how this compares with Microsoft's Small Cheri 
+  (Technical report coming up -- as of Oct 24 2022) *)
+  Definition representable_length (len : N) : N :=
+    let mask:N := representable_alignment_mask len in
+    let nmask:Z := Value.bitwise_complement (Z.of_N mask) in
+    let result:Z := Z.land (Z.add (Z.of_N len) nmask) (Z.of_N mask) in 
+      Z.to_N result.
 
-  Definition cap_seal_indirect_entry (c : t) : t := c. (* TODO: looks like it is not implemented yet *)
+  Definition make_cap (value : Value.t) (otype : ObjType.t) (bounds : Bounds.t) (perms : Permissions.t) : t :=
+    let new_cap := cap_cU () in 
+    let perms_to_clear := list_bool_to_bv (map negb (bv_to_list_bool perms)) in 
+    let new_cap := cap_narrow_perms new_cap perms_to_clear in 
+    let new_cap := cap_narrow_bounds new_cap bounds in 
+    let new_cap := cap_set_value new_cap value in 
+      cap_set_objtype new_cap otype.
+    
+  (* Should we check that size is not too large? *)
+  Definition alloc_cap (a_value : Value.t) (size : Value.t) : t :=
+    make_cap 
+      a_value 
+      cap_SEAL_TYPE_UNSEALED 
+      (Bounds.of_Zs (bv_to_Z_unsigned a_value, Z.add (bv_to_Z_unsigned a_value) (bv_to_Z_unsigned size)))
+      (Permissions.perm_alloc).
+    
+  Definition alloc_fun (a_value : Value.t) : t :=
+    make_cap 
+      a_value 
+      cap_SEAL_TYPE_RB 
+      (Bounds.of_Zs (bv_to_Z_unsigned a_value, Z.succ (Z.succ (bv_to_Z_unsigned a_value)))) 
+      Permissions.perm_alloc_fun.
 
-  Definition cap_seal_indirect_entry_pair (c : t) : t := c. (* TODO: looks like it is not implemented yet *)
+  Definition value_compare (cap1 cap2 : t) : comparison :=
+    if (cap_get_value cap1 =? cap_get_value cap2)%stdpp then Eq
+    else if (cap_get_value cap1 <? cap_get_value cap2) then Lt
+    else Gt.
 
-  Definition cap_set_flags (c : t) (f : list bool) : t :=
-    invalidate_if_sealded (with_flags f c).
+  Definition exact_compare (cap1 cap2 : t) : comparison :=
+    if (cap1 =? cap2) then Eq 
+    else if (cap1 <? cap2) then Lt 
+    else Gt.
 
-  Definition cap_unseal (c : t) (k : t) : t :=
-    with_obj_type cap_SEAL_TYPE_UNSEALED c. (* TODO: looks like it is not implemented yet *)
+  Definition cap_vaddr_representable (c : t) (a : Value.t) : bool :=
+    CapIsRepresentable (bv_to_mword c) (bv_to_mword a).
+  
+  Definition cap_bounds_representable_exactly (cap : t) (bounds : Bounds.t) : bool :=
+    let '(base, limit) := bounds in
+    let len := Z.sub (bv_to_Z_unsigned limit) (bv_to_Z_unsigned base) in
+    let base' : (bv Value.len) := 
+      Z_to_bv Value.len (bv_to_Z_unsigned base) in 
+    let len' := mword_of_int (len:=Z.of_N Bounds.bound_len) len in 
+    let new_cap : (bv _) := cap_set_value cap base' in
+    let new_cap : (mword _) := CapSetBounds (bv_to_mword new_cap) len' true in
+    CapIsTagSet new_cap.
 
+  Definition cap_is_null_derived (cap : t) : bool :=
+    let a := cap_get_value cap in
+    let c0 := cap_c0 () in
+    let c' := cap_set_value c0 a in
+    cap =? c'.
+    
+  (* Extracted from https://github.com/vzaliva/cerberus/blob/master/coq/Utils.v *)  
+  Definition bool_bits_of_bytes (bytes : list ascii): list bool
+  :=
+  let ascii_to_bits (x:ascii) :=
+    match x with
+    | Ascii a0 a1 a2 a3 a4 a5 a6 a7 => [a0; a1; a2; a3; a4; a5; a6; a7]
+    end
+  in
+  List.fold_left (fun l a => List.app l (ascii_to_bits a)) bytes [].  
 
+  (* Definition bool_bits_of_bytes (bytes : list ascii): list bool :=
+    let ascii_to_bits (x:ascii) :=
+      match x with
+      | Ascii a0 a1 a2 a3 a4 a5 a6 a7 => [a0; a1; a2; a3; a4; a5; a6; a7]
+      end in 
+    List.flat_map ascii_to_bits bytes. *)
+   
   (* Internal helper function to conver between Sail bytes ([memory_byte])
      and Cerberus bytes ([ascii]). *)
   Definition memory_byte_to_ascii (b:memory_byte) : option ascii :=
@@ -504,13 +701,29 @@ Module MorelloCapability <:
     | _ => None
     end.
 
-  Program Definition encode (isexact : bool) (c : t) : option ((list ascii) * bool) :=
-    let w := encode_to_word isexact c in
-    let tag := CapIsTagSet w in
-    (* strip tag bit *)
-    let bits := bits_of w in
-    let w1 := vec_of_bits (List.tail bits) in
-    match mem_bytes_of_bits w1 with
+  (* Extracted from https://github.com/vzaliva/cerberus/blob/master/coq/Utils.v *)
+  (* could be generalized as monadic map, or implemente as compistion
+   of [map] and [sequence]. *)
+  Fixpoint try_map {A B:Type} (f : A -> option B) (l:list A) : option (list B)
+  :=
+  match l with
+  | [] => Some []
+  | a :: t =>
+      match f a with
+      | Some b =>
+          match try_map f t with
+          | Some bs =>  Some (b :: bs)
+          | None => None
+          end
+      | None => None
+      end
+  end.
+
+  Definition encode (isexact : bool) (cap : t) : option ((list ascii) * bool) :=
+    let tag : bool := cap_is_valid cap in 
+    let cap_bits := bits_of (bv_to_mword cap) in 
+    let w : (mword _) := vec_of_bits (List.tail cap_bits) in
+    match mem_bytes_of_bits w with
     | Some bytes =>
         match try_map memory_byte_to_ascii bytes with
         | Some chars => Some ((List.rev chars), tag)
@@ -519,56 +732,548 @@ Module MorelloCapability <:
     | None => None
     end.
 
-  Definition representable_alignment_mask (len: Z) : Z :=
-    let len' := mword_of_int (len:=Z.of_nat vaddr_bits) len in
-    let mask := CapGetRepresentableMask len' in
-    uwordToZ mask.
+  Definition decode (bytes : list ascii) (tag : bool) : option (bv Cap.len) :=
+    if Nat.eq_dec (List.length bytes) 16%nat then
+      let bits : (list bool) := tag::(bool_bits_of_bytes bytes) in
+      let bitsu := List.map bitU_of_bool bits in
+      let w : (mword _) := vec_of_bits bitsu in
+      (* Some (mword_to_bv w) *) (* This requires the proof below, but makes tests harder *)
+      let z : Z := mword_to_Z_unsigned w in 
+      let c : option (bv Cap.len) := Z_to_bv_checked Cap.len z in 
+      c
+    else
+      None.
+    (* Next Obligation.      
+      intros. assert (P: length bytes = 16%nat).
+      - unfold bytes. rewrite rev_length. apply e.
+      - assert (Q: length (bool_bits_of_bytes bytes) = 128%nat).
+        + assert (X: forall (bs:list ascii), length (bool_bits_of_bytes bs) = (8 * (length bs))%nat).
+          { induction bs as [| h tl HInd].
+          - reflexivity.
+          - simpl bool_bits_of_bytes. rewrite app_length. destruct h.
+            simpl length. rewrite HInd. 
+            assert (T: (8 + 8 * base.length tl)%nat = (8*1 + 8 * base.length tl)%nat).
+            + reflexivity.
+            + rewrite T. rewrite <- mult_plus_distr_l. reflexivity. }
+          rewrite X. rewrite P. reflexivity.
+          + assert (R: length bits = 129%nat). 
+            -- unfold bits. rewrite list.cons_length. rewrite Q. reflexivity. 
+            -- unfold bitsu. unfold length_list. rewrite map_length. rewrite R. reflexivity.
+    Defined. *)  
 
-  Definition representable_length (len : Z) : Z :=
-    let mask := representable_alignment_mask len in
-    let nmask := MorelloAddr.bitwise_complement mask in
-    Z.land (Z.add len nmask) mask.
+  Definition eqb (cap1:t) (cap2:t) : bool := (cap1 =? cap2)%stdpp.
 
-  Definition eqb (a b : t) : bool :=
-    eq_vec (encode_to_word true a) (encode_to_word true b).
+  Definition to_string (cap:t) : string :=
+    String.hex_string_of_int (bv_to_Z_unsigned cap).
 
-  Definition value_compare (x y : t) : comparison :=
-    Z.compare x.(value) y.(value).
-
-  (* TODO: this implmenetation seems to be incomplete. Must compare
-     all other fields. One idea is to convert both arguments to bit
-     vectors and compare them. This would work if the ordering imposed
-     by this function only used when indexing hash maps with
-     capabilities as keys.
-
-     If used for something else we need to see if this ordering is
-     compatible with one imposed by [value_compare]. E.g.  *)
-  Definition exact_compare (x y : t) : comparison :=
-    match Bool.compare x.(valid) y.(valid) with
-    | Eq => value_compare x y
-    | Lt => Lt
-    | Gt => Gt
-    end.
-
-  Definition cap_is_null_derived (c : t) : bool :=
-    let a := cap_get_value c in
-    let c0 := cap_c0 tt in
-    let c' := cap_set_value c0 a in
-    eqb c c'.
-
-  Lemma eqb_exact_compare: forall a b, eqb a b = true <-> exact_compare a b = Eq.
-  Proof.
-    (* could not be proven under current definition of eqb! *)
-  Admitted.
+  (* Could also implement a prettier to_string that produces something like
+    { valid: yes
+      value: 0xF...1
+      base: 0xF...
+      limit: ...
+      seal: RB
+      permissions: Load,Store,Execute
+      flags: 10010...  
+    }   *)  
 
   Lemma eqb_value_compare: forall a b, eqb a b = true -> value_compare a b = Eq.
-  Proof.
-    (* could not be proven under current definition of eqb! *)
-  Admitted.
+  Proof. intros. unfold eqb in H. assert (P: a = b).
+    { unfold eq in H. rewrite -> Z.eqb_eq in H. apply bv_eq. apply H. }
+    rewrite <- P. unfold value_compare. unfold eq. rewrite Z.eqb_refl. reflexivity. Qed.
+        
+  Lemma eqb_exact_compare: forall a b, eqb a b = true <-> exact_compare a b = Eq.
+  Proof. split.
+    - unfold eqb. unfold exact_compare. intros. rewrite H. reflexivity. 
+    - unfold eqb. unfold exact_compare. destruct (a =? b).
+      + reflexivity.
+      + destruct (b >? a). 
+        { discriminate. } { discriminate. }
+    Qed.
+    
+End Cap.  
 
-  Definition to_string (c: t) : string := "TODO".
 
-  Definition strfcap (formats : string) (capability : t) : option string :=
-    None. (* TODO *)
+Module test_cap_getters_and_setters.
 
-End MorelloCapability.
+  Import Cap.
+
+  Definition c1:Cap.t := mword_to_bv (concat_vec (Ones 19) (Zeros 110)). (* A valid universal-permission cap = 1^{19}0^{110} *)
+  Definition c2:Cap.t := mword_to_bv (concat_vec (Ones 3) (Zeros 126)). (* A valid cap with Load and Store perms *)
+  Definition c3:Cap.t := Cap.of_Z 0x1fc000000333711170000000012342222. (* The default cap on https://www.morello-project.org/capinfo *)
+  Definition c4:Cap.t := Cap.of_Z 0x1fc000000399700070000000012342222. (* The bounds in this cap subsume those of c3 *)
+  Definition c5:Cap.t := Cap.of_Z 0x1fb000000377700070011111111113333. (* Cap breakdown: https://www.morello-project.org/capinfo?c=0x1%3Afb00000037770007%3A0011111111113333 *)
+  Definition c6:Cap.t := Cap.of_Z 0x1fb0000007a4700000000000000003333. (* Cap breakdown: https://www.morello-project.org/capinfo?c=0x1%3Afb0000007a470000%3A0000000000003333 *)
+  
+  Program Definition flags1:Cap.Flags := exist _ [false; false; false; false; false; false; false; false] _. 
+    Next Obligation. reflexivity. Defined.
+  Program Definition flags2:Cap.Flags := exist _ [false; true; false; true; false; true; false; true] _. 
+    Next Obligation. reflexivity. Defined.
+    
+  Definition perm_Load : list bool := Permissions.make_permissions [Permissions.Load_perm].
+  Definition perm_Load_Store : list bool := Permissions.make_permissions [Permissions.Load_perm; Permissions.Store_perm].
+  Definition perm_Load_Execute : list bool := Permissions.make_permissions [Permissions.Load_perm; Permissions.Execute_perm].
+  
+  Example is_valid_test_1 :
+    cap_is_valid c1 = true.
+    Proof. reflexivity. Qed.
+
+  Example is_valid_test_2 :
+    cap_is_valid (cap_c0 ()) = false.
+    Proof. reflexivity. Qed.
+
+  Example is_valid_test_3 :
+    cap_is_valid c5 = true.
+    Proof. reflexivity. Qed.
+
+  Example is_valid_test_4 :
+    cap_is_valid c2 = true.
+    Proof. reflexivity. Qed.
+
+  Example value_test_1 : 
+    let value:Value.t := Value.of_Z 50 in
+    value = cap_get_value (cap_set_value c1 value).
+    Proof. reflexivity. Qed. 
+
+  Example flags_test_1 : flags1 = cap_get_flags c1.
+    Proof. reflexivity. Qed.
+
+  Example flags_test_2 : flags2 = cap_get_flags (cap_set_flags c1 flags2).
+    Proof. reflexivity. Qed. 
+  
+  Import Permissions.
+  
+  Example permissions_test_1 : 
+    Permissions.perm_Universal = cap_get_perms c1.
+    Proof. reflexivity. Qed.
+
+  Example permissions_test_2 : 
+    let mask : Permissions.t := list_bool_to_bv (map negb perm_Load_Store) in
+    list_bool_to_bv perm_Load_Store = cap_get_perms (cap_narrow_perms c1 mask).
+    Proof. reflexivity. Qed.
+
+  Example permissions_test_3 : 
+    let mask : Permissions.t := list_bool_to_bv (map negb perm_Load_Store) in
+    let cap := (cap_narrow_perms c1 mask) in 
+    let mask : Permissions.t := list_bool_to_bv (map negb perm_Load_Execute) in
+    list_bool_to_bv perm_Load = cap_get_perms (cap_narrow_perms cap mask).
+    Proof. vm_compute. reflexivity. Qed.
+
+  Example permissions_test_4 : 
+    let mask : Permissions.t := list_bool_to_bv (map negb (make_permissions [Load_perm; Execute_perm])) in  
+    let capA := (cap_narrow_perms c1 mask) in     
+    let perms : Permissions.t := Permissions.perm_Universal in 
+    let perms := perm_clear_store_cap perms in 
+    let perms := perm_clear_store perms in 
+    let perms := perm_clear_global perms in 
+    let perms := perm_clear_executive perms in 
+    let perms := perm_clear_seal perms in 
+    let perms := perm_clear_load_cap perms in 
+    let perms := perm_clear_store_local_cap perms in 
+    let perms := perm_clear_system_access perms in 
+    let perms := perm_clear_unseal perms in 
+    let perms := perm_clear_branch_sealed_pair perms in 
+    let perms := perm_clear_mutable_load perms in 
+    let perms := perm_clear_compartment_ID perms in 
+    let perms := perm_clear_user4 perms in 
+    let perms := perm_clear_user3 perms in 
+    let perms := perm_clear_user2 perms in 
+    let perms := perm_clear_user1 perms in 
+    let perms := Permissions.of_list (map negb (Permissions.to_list perms)) in
+    let capB := (cap_narrow_perms c1 (match perms with Some p => p | None => Permissions.perm_Universal end)) in
+    capA = capB.
+    Proof. vm_compute. reflexivity. Qed.
+
+  Example get_and_user_perms_test_1 : 
+    let user_perms_A : (list bool) := get_user_perms (cap_get_perms (cap_cU ())) in 
+    let user_perms_A := [ nth 0 user_perms_A false; negb (nth 1 user_perms_A false);
+                        nth 2 user_perms_A false; negb (nth 3 user_perms_A false) ] in 
+    let user_perms_B : Permissions.t := 
+      perm_and_user_perms (cap_get_perms (cap_cU ())) user_perms_A in
+      user_perms_A = [true; false; true; false] /\
+      get_user_perms user_perms_B = user_perms_A.
+    Proof. vm_compute. split. reflexivity. reflexivity. Qed. 
+ 
+  Example eqb_and_narrow_perm_test_1 :
+    let mask : Permissions.t := list_bool_to_bv (map negb perm_Load_Store) in
+    (c2 = (cap_narrow_perms c1 mask))%stdpp.
+    Proof. vm_compute. reflexivity. Qed.
+
+  Example bounds_representable_exactly_test_1 :
+    let bounds : Bounds.t := 
+      (Z_to_bv Bounds.bound_len 305402128, Z_to_bv Bounds.bound_len 305427248) in (* the bounds of c3, which we know is representable *) 
+    cap_bounds_representable_exactly c4 bounds = true.
+    Proof. reflexivity. Qed. 
+      
+  Example bounds_representable_exactly_test_2 :
+    let bounds : Bounds.t := 
+      (Z_to_bv Bounds.bound_len 305402128, Z_to_bv Bounds.bound_len 306427248) in (* now we changed the common part of the bounds *) 
+    cap_bounds_representable_exactly c4 bounds = false.
+    Proof. reflexivity. Qed. 
+  
+  Example narrow_exact_and_get_bounds_test_1 : 
+    (* The bounds of capability c5 are         (0x0011111111110000, 0x00011111111117770). *)
+    let '(new_base,new_limit) := Bounds.of_Zs  (0x0011111111113330, 0x00011111111117440) in 
+    (* We can see new_bounds can be represented exactly from cap5: https://www.morello-project.org/capinfo?c=0x1%3Afb00000034473337%3A1011111111113333 *)
+    let new_cap := cap_narrow_bounds_exact c5 (new_base,new_limit) in 
+    let '(base_set,limit_set,isExpValid) := cap_get_bounds new_cap in 
+    isExpValid = true /\ (base_set = new_base) /\ (limit_set =? new_limit) = true
+    /\ cap_is_valid c5 = true /\ cap_is_valid new_cap = true.
+    Proof. vm_compute. split. reflexivity. split. reflexivity. split. reflexivity. 
+      split. reflexivity. reflexivity. Qed.
+  
+  Example seal_and_unseal_test_1 :
+    (* c6 has Seal and Unseal permissions and its value is <= the largest objtype. *) 
+    let sealed_cap := cap_seal c3 c6 in
+    let unsealed_sealed_cap := cap_unseal sealed_cap c6 in 
+    (cap_is_valid sealed_cap) = true /\ (cap_is_sealed sealed_cap) = true 
+    /\ (cap_get_obj_type sealed_cap) = (cap_get_value c6) 
+    /\ (cap_is_valid unsealed_sealed_cap) = true /\ (cap_is_unsealed unsealed_sealed_cap) = true.
+    Proof. vm_compute. repeat ( split; try reflexivity ). Qed.
+
+  Example seal_entry_test_1 : 
+    let sealed_cap := cap_seal_entry c4 in 
+    let sealed_sealed_cap := cap_seal_entry sealed_cap in 
+    let sealed_invalid_cap := cap_seal_entry (cap_invalidate c4) in 
+    (cap_is_sealed sealed_cap) = true /\ (cap_is_valid sealed_cap) = true 
+    /\ (cap_get_obj_type sealed_cap = SealType.sealed_entry_ot)
+    /\ (cap_is_invalid sealed_sealed_cap) = true /\ (cap_is_invalid sealed_invalid_cap) = true.
+    Proof. repeat ( split; try reflexivity ). Qed. 
+
+  Example seal_indirect_entry_test_1 : 
+    let sealed_cap := cap_seal_indirect_entry c3 in 
+    let sealed_sealed_cap := cap_seal_indirect_entry sealed_cap in 
+    let sealed_invalid_cap := cap_seal_indirect_entry (cap_invalidate c3) in 
+    (cap_is_sealed sealed_cap) = true /\ (cap_is_valid sealed_cap) = true 
+    /\ (cap_get_obj_type sealed_cap = SealType.sealed_indirect_entry_ot)
+    /\ (cap_is_invalid sealed_sealed_cap) = true /\ (cap_is_invalid sealed_invalid_cap) = true.
+    Proof. repeat ( split; try reflexivity ). Qed.
+      
+  Example seal_indirect_entry_pair_test_1 : 
+    let sealed_cap := cap_seal_indirect_entry_pair c5 in 
+    let sealed_sealed_cap := cap_seal_indirect_entry_pair sealed_cap in 
+    let sealed_invalid_cap := cap_seal_indirect_entry_pair (cap_invalidate c5) in 
+    (cap_is_sealed sealed_cap) = true /\ (cap_is_valid sealed_cap) = true 
+    /\ (cap_get_obj_type sealed_cap = SealType.sealed_indirect_entry_pair_ot)
+    /\ (cap_is_invalid sealed_sealed_cap) = true /\ (cap_is_invalid sealed_invalid_cap) = true.
+    Proof. repeat ( split; try reflexivity ). Qed.
+        
+  Example alloc_cap_test_1 : 
+    let value := Value.of_Z 1024 in 
+    let new_cap := alloc_cap value (Value.of_Z 2048) in 
+    (cap_is_valid new_cap) /\ (cap_get_value new_cap) = value 
+    /\ (cap_is_in_bounds new_cap) /\ (cap_is_sealed new_cap) = false 
+    /\ (cap_get_seal new_cap) = SealType.Cap_Unsealed 
+    /\ (cap_get_perms new_cap) = Permissions.perm_alloc
+    /\ (cap_get_bounds new_cap) = (Bounds.of_Zs (1024,3072), true).
+    Proof. vm_compute. repeat (split; try reflexivity). Qed. 
+  
+  Example alloc_cap_test_2 : 
+    let value := Value.of_Z 0xffffffffffffffff in (* 16 f's = the largest Value possible *)
+    let new_cap := alloc_cap value (Value.of_Z 1) in 
+    (cap_is_valid new_cap) = true /\ (cap_get_value new_cap) = value 
+    /\ (cap_is_in_bounds new_cap) /\ (cap_is_sealed new_cap) = false 
+    /\ (cap_get_seal new_cap) = SealType.Cap_Unsealed 
+    /\ (cap_get_perms new_cap) = Permissions.perm_alloc
+    /\ (cap_get_bounds new_cap) = (Bounds.of_Zs (0xffffffffffffffff,0x10000000000000000), true).
+    Proof. vm_compute. repeat (split; try reflexivity). Qed. 
+
+  Example alloc_cap_test_3 : 
+    let value := Value.of_Z 0x10000000000000000 in (* 1 past the largest Value possible; it gets passed as just 0 *)
+    let new_cap := alloc_cap value (Value.of_Z 1) in 
+    (cap_is_valid new_cap) = true 
+    /\ (cap_is_in_bounds new_cap) = true (* it's in bounds bc these are (0,1) *)
+    /\ (cap_is_sealed new_cap) = false /\ (cap_get_seal new_cap) = SealType.Cap_Unsealed 
+    /\ (cap_get_perms new_cap) = Permissions.perm_alloc  
+    /\ (cap_get_bounds new_cap) <> (Bounds.of_Zs (0x10000000000000000,0x10000000000000001), true).
+    Proof. vm_compute. repeat (split; try reflexivity). intros H. discriminate H. Qed.
+
+  Example alloc_cap_test_4 : 
+    let value := Value.of_Z 0xffffffffffffff in (* 14 f's *)
+    let new_cap := alloc_cap value (Value.of_Z 0xfff) in (* this sends the limit above the max limit allowed *)
+    (cap_is_invalid new_cap) /\ (cap_is_not_in_bounds new_cap)
+    /\ (cap_is_sealed new_cap) = false /\ (cap_get_seal new_cap) = SealType.Cap_Unsealed 
+    /\ (cap_get_perms new_cap) = Permissions.perm_alloc  
+    /\ (cap_get_bounds new_cap) <> (Bounds.of_Zs (0xffffffffffffff,0xfffffffffffffffff), true).
+    Proof. vm_compute. repeat (split; try reflexivity). intro H. discriminate H. Qed.   
+          
+  Example alloc_fun_test_1 : 
+    let value := Value.of_Z 1024 in 
+    let new_cap := alloc_fun value in 
+    (cap_is_valid new_cap) = true /\ (cap_get_value new_cap) = value 
+      /\ (cap_is_sealed new_cap) = true /\ (cap_get_seal new_cap) = SealType.Cap_SEntry 
+      /\ (cap_get_perms new_cap) = Permissions.perm_alloc_fun
+      /\ (cap_get_bounds new_cap) = (Bounds.of_Zs (1024,1026), true).
+    Proof. repeat (split; try reflexivity). Qed. 
+
+  Example cap_is_null_derived_test_1 : 
+    let new_cap := cap_c0 () in 
+    let new_cap := cap_set_value new_cap (Value.of_Z 512) in 
+    cap_is_null_derived new_cap.
+    Proof. vm_compute. reflexivity. Qed.
+      
+  Example cap_is_null_derived_test_2 : 
+    let new_cap := cap_cU () in 
+    let new_cap := cap_set_value new_cap (Value.of_Z 512) in 
+    (cap_is_null_derived new_cap) = false.
+    Proof. vm_compute. reflexivity. Qed.
+
+  Example encode_and_decode_test_1 :     
+    let tester := fun cap:Cap.t => 
+      let encoded_cap : option ((list ascii) * bool) := encode true cap in 
+      let decoded_cap : option Cap.t :=
+        match encoded_cap with 
+          Some (l,tag) => (decode l tag) | None => None
+        end in 
+      let c_ : Cap.t := 
+        match decoded_cap with 
+          Some c => c | None => cap_c0 () 
+        end in 
+        (c_ =? cap) = true in
+      tester c1 /\ tester c2 /\ tester c3 /\ tester c4 /\ tester c5 /\ tester c6.
+    Proof. vm_compute. repeat (split; try reflexivity). Qed.
+ 
+End test_cap_getters_and_setters.
+
+Module PermissionsZ <: Permission. 
+  Definition t := Z. 
+
+  Definition user_perms_len := Permissions.user_perms_len.
+
+  Definition has_global_perm (perms:t) : bool := 
+    Permissions.has_global_perm (Permissions.of_Z perms).
+   
+  Definition has_execute_perm (perms:t) : bool := 
+    Permissions.has_execute_perm (Permissions.of_Z perms).
+  Definition has_ccall_perm (perms:t) : bool := 
+    Permissions.has_ccall_perm (Permissions.of_Z perms).
+  Definition has_load_perm (perms:t) : bool := 
+    Permissions.has_load_perm (Permissions.of_Z perms).
+  Definition has_load_cap_perm (perms:t) : bool := 
+    Permissions.has_load_cap_perm (Permissions.of_Z perms).
+  Definition has_seal_perm (perms:t) : bool := 
+    Permissions.has_seal_perm (Permissions.of_Z perms).
+  Definition has_store_perm (perms:t) : bool := 
+    Permissions.has_store_perm (Permissions.of_Z perms).
+  Definition has_store_cap_perm (perms:t) : bool := 
+    Permissions.has_store_cap_perm (Permissions.of_Z perms).
+  Definition has_store_local_cap_perm (perms:t) : bool := 
+    Permissions.has_store_local_cap_perm (Permissions.of_Z perms).
+  Definition has_system_access_perm (perms:t) : bool := 
+    Permissions.has_system_access_perm (Permissions.of_Z perms).
+  Definition has_unseal_perm (perms:t) : bool := 
+    Permissions.has_unseal_perm (Permissions.of_Z perms).
+  
+  Definition get_user_perms (perms:t) : list bool :=
+    Permissions.get_user_perms (Permissions.of_Z perms).
+ 
+
+  Definition perm_clear_global (perms:t) : t := 
+    bv_to_Z_unsigned (Permissions.perm_clear_global (Permissions.of_Z perms)).
+  
+  Definition perm_clear_execute (perms:t) : t := bv_to_Z_unsigned (Permissions.perm_clear_execute (Permissions.of_Z perms)).
+  Definition perm_clear_ccall (perms:t) : t := bv_to_Z_unsigned (Permissions.perm_clear_ccall (Permissions.of_Z perms)).
+  Definition perm_clear_load (perms:t) : t := bv_to_Z_unsigned (Permissions.perm_clear_load (Permissions.of_Z perms)).
+  Definition perm_clear_load_cap (perms:t) : t := bv_to_Z_unsigned (Permissions.perm_clear_load_cap (Permissions.of_Z perms)).
+  Definition perm_clear_seal (perms:t) : t := bv_to_Z_unsigned (Permissions.perm_clear_seal (Permissions.of_Z perms)).
+  Definition perm_clear_store (perms:t) : t := bv_to_Z_unsigned (Permissions.perm_clear_store (Permissions.of_Z perms)).
+  Definition perm_clear_store_cap (perms:t) : t := bv_to_Z_unsigned (Permissions.perm_clear_store_cap (Permissions.of_Z perms)).
+  Definition perm_clear_store_local_cap (perms:t) : t := bv_to_Z_unsigned (Permissions.perm_clear_store_local_cap (Permissions.of_Z perms)).
+  Definition perm_clear_system_access (perms:t) : t := bv_to_Z_unsigned (Permissions.perm_clear_system_access (Permissions.of_Z perms)).
+  Definition perm_clear_unseal (perms:t) : t := bv_to_Z_unsigned (Permissions.perm_clear_unseal (Permissions.of_Z perms)).
+  
+  (** perform bitwise AND of user permissions *)
+  Definition perm_and_user_perms (perms:t) (l:list bool) : t := 
+    bv_to_Z_unsigned (Permissions.perm_and_user_perms (Permissions.of_Z perms) l).
+ 
+  (** null permission *)
+  Definition perm_p0: t := bv_to_Z_unsigned (Permissions.perm_p0).
+
+  (** permissions for newly allocated region *)
+  Definition perm_alloc: t := bv_to_Z_unsigned (Permissions.perm_alloc).
+
+  (** permissions for newly allocated function *)
+  Definition perm_alloc_fun: t := bv_to_Z_unsigned (Permissions.perm_alloc_fun).
+
+  (* --- Utility methods --- *)
+
+  Definition to_string (perms:t) : string := Permissions.to_string (Permissions.of_Z perms).
+
+  (* raw permissoins in numeric format *)
+  Definition to_raw (perms:t) : Z := perms.
+
+  (* Initialize from list of boolean. The size and
+     contents of the list is implementation-specific.
+     Returns None in case of error *)
+  Definition of_list (l:list bool) : option t := 
+    match Permissions.of_list l with 
+      Some c => Some (bv_to_Z_unsigned c) | None => None
+    end.
+
+  (* inverse of [of_list] *)
+  Definition to_list (perms:t) : list bool := Permissions.to_list (Permissions.of_Z perms).
+End PermissionsZ.
+
+Module ValueZ <: VADDR.
+  Definition t := Z.
+
+  Definition bitwise_complement (a:Z) : Z := Value.bitwise_complement a.
+    
+  Definition eqb (v1:t) (v2:t) : bool := Value.eqb (Value.of_Z v1) (Value.of_Z v2).
+  Definition ltb (v1:t) (v2:t) : bool := Value.ltb (Value.of_Z v1) (Value.of_Z v2).
+  Definition leb (v1:t) (v2:t) : bool := Value.leb (Value.of_Z v1) (Value.of_Z v2).
+  
+  Definition ltb_irref: forall a:t, ltb a a = false.
+  Proof. intros. unfold ltb. unfold Value.ltb. unfold lt. rewrite Z.ltb_irrefl. reflexivity. Qed. 
+
+  Definition of_Z (z:Z) := z.
+  Definition to_Z (v:t) := v.
+  
+End ValueZ.
+
+
+Module ObjTypeZ <: OTYPE.
+  Definition t := Z.  
+End ObjTypeZ.
+
+
+Module BoundsZ <: VADDR_INTERVAL(ValueZ).
+  Definition t := (Z * Z)%type.
+  
+  Definition address_is_in_interval (bounds:t) (value:ValueZ.t) : bool :=
+    Bounds.address_is_in_interval (Bounds.of_Zs bounds) (Value.of_Z value). 
+
+  (* Vadim: is this what we want? *)
+  Definition ltb (a b:t) := Bounds.ltb (Bounds.of_Zs a) (Bounds.of_Zs b).
+
+End BoundsZ. 
+
+Module MorelloCap <: Capability (ValueZ) (ObjTypeZ) (SealType) (BoundsZ) (PermissionsZ).
+  Definition t := Cap.t.
+  
+  (* Definition vaddr_bits := sizeof_vaddr * 8. *)
+  Definition sizeof_vaddr := Cap.sizeof_vaddr. (* in bytes *)
+  Definition min_vaddr := Value.to_Z Cap.min_vaddr.  
+  Definition max_vaddr := Value.to_Z Cap.max_vaddr.
+
+  Definition cap_c0 := Cap.cap_c0.
+  
+  Definition cap_flags_len := Cap.cap_flags_len.
+  Definition Flags := Cap.Flags.
+
+  Definition cap_get_value (cap:t) : ValueZ.t := 
+    Value.to_Z (Cap.cap_get_value cap). 
+  
+  Definition cap_get_obj_type (cap:t) : ObjTypeZ.t := 
+    ObjType.to_Z (Cap.cap_get_obj_type cap).
+
+  Definition cap_get_bounds (cap:t) : BoundsZ.t * bool :=
+    let (bounds,tag) := Cap.cap_get_bounds cap in 
+    (Bounds.to_Zs bounds, tag).
+
+  Definition cap_get_offset (cap:t) : Z := Cap.cap_get_offset cap.
+      
+  Definition cap_get_seal (cap:t) : SealType.t := Cap.cap_get_seal cap. 
+  
+  (* The flags are the top byte of the value. *)
+  Definition cap_get_flags (cap:t) : Flags := 
+    Cap.cap_get_flags cap. 
+
+  Definition cap_get_perms (cap:t) : PermissionsZ.t :=
+    Permissions.to_Z (Cap.cap_get_perms cap).
+    
+  Definition cap_invalidate (cap:t) : t := Cap.cap_invalidate cap.
+
+  Definition cap_set_value (cap:t) (value:ValueZ.t) : t :=
+    Cap.cap_set_value cap (Value.of_Z value).
+    
+  Definition cap_set_flags := Cap.cap_set_flags.
+  
+  Definition cap_set_objtype (cap:t) (ot:ObjTypeZ.t) : t :=
+    Cap.cap_set_objtype cap (ObjType.of_Z ot).
+    
+  Definition cap_is_sealed := Cap.cap_is_sealed.
+
+  (* [perms] must contain [1] for permissions to be cleared and [0] for those to be kept *)
+  Definition cap_narrow_perms (cap:t) (perms:PermissionsZ.t) : t :=
+    Cap.cap_narrow_perms cap (Permissions.of_Z perms).
+    
+  Definition cap_narrow_bounds (cap : t) (bounds : BoundsZ.t) : t :=
+    Cap.cap_narrow_bounds cap (Bounds.of_Zs bounds).
+
+  Definition cap_narrow_bounds_exact (cap : t) (bounds : BoundsZ.t) : t :=
+    Cap.cap_narrow_bounds_exact cap (Bounds.of_Zs bounds).
+
+  Definition cap_is_valid := Cap.cap_is_valid.
+
+  Definition cap_seal := Cap.cap_seal.
+  
+  Definition cap_unseal := Cap.cap_unseal.
+
+  (* For sealing with RB *)
+  Definition cap_seal_entry := Cap.cap_seal_entry.
+  
+  (* For sealing with LB *)
+  Definition cap_seal_indirect_entry := Cap.cap_seal_indirect_entry.
+
+  (* For sealing with LPB *)  
+  Definition cap_seal_indirect_entry_pair := Cap.cap_seal_indirect_entry_pair.
+    
+  (* Confirm the type of the function is ok *)  
+  Definition representable_alignment_mask := Cap.representable_alignment_mask.
+
+  (* Will need to see how this compares with Microsoft's Small Cheri 
+  (Technical report coming up -- as of Oct 24 2022) *)
+  Definition representable_length := Cap.representable_length.
+    
+  (* Should we check that size is not too large? *)
+  Definition alloc_cap (a_value : ValueZ.t) (size : ValueZ.t) : t :=
+    Cap.alloc_cap (Value.of_Z a_value) (Value.of_Z size).
+  
+  Definition alloc_fun (a_value : ValueZ.t) : t :=
+    Cap.alloc_fun (Value.of_Z a_value).
+
+  Definition value_compare := Cap.value_compare.
+
+  Definition exact_compare := Cap.exact_compare.
+
+  Definition cap_vaddr_representable (c : t) (a : ValueZ.t) : bool :=
+    Cap.cap_vaddr_representable c (Value.of_Z a).
+  
+  Definition cap_bounds_representable_exactly (cap : t) (bounds : BoundsZ.t) : bool :=
+    Cap.cap_bounds_representable_exactly cap (Bounds.of_Zs bounds).
+
+  Definition cap_is_null_derived := Cap.cap_is_null_derived.
+  
+  Definition encode := Cap.encode.
+
+  Definition decode := Cap.decode.
+
+  Definition eqb := Cap.eqb.
+
+  Definition to_string := Cap.to_string.
+
+  (* Could also implement a prettier to_string that produces something like
+    { valid: yes
+      value: 0xF...1
+      base: 0xF...
+      limit: ...
+      seal: RB
+      permissions: Load,Store,Execute
+      flags: 10010...  
+    }   *)  
+
+  Lemma eqb_value_compare: forall (a b:t), eqb a b = true -> value_compare a b = Eq.
+  Proof. intros. unfold eqb in H. assert (P: a = b).
+    { unfold Cap.eqb in H. unfold eq in H. rewrite -> Z.eqb_eq in H. apply bv_eq. apply H. }
+    rewrite <- P. unfold value_compare. unfold Cap.value_compare. unfold eq. rewrite Z.eqb_refl. reflexivity. Qed.
+        
+  Lemma eqb_exact_compare: forall a b, eqb a b = true <-> exact_compare a b = Eq.
+  Proof. split.
+    - unfold eqb. unfold Cap.eqb. unfold exact_compare. unfold Cap.exact_compare. intros. rewrite H. reflexivity. 
+    - unfold eqb.  unfold Cap.eqb. unfold exact_compare. unfold Cap.exact_compare. destruct (a =? b).
+      + reflexivity.
+      + destruct (b >? a). 
+        { discriminate. } { discriminate. }
+    Qed.
+
+End MorelloCap.
